comments and policy problem

src/NegotiationManifest.v
@@ -1,9 +1,5 @@
-(* Functions surrounding Negotiation for DEMO 
-
-   Roughly, code will: 
-   1. pass in protocol
-   2. ensure protocol is sound and executable 
-
+(* 
+  Negotiation over Manifests (NOT enviornments)
 *)
 
 Require Import Manifest. 
@@ -47,32 +43,28 @@ Definition System := list Environment.
   * REASONING ABOUT MANIFESTS
 *****************************)
 
-(** Within the enviornment [e], does the AM at place [k] have ASP [a]? *)
-
-Search "In". 
-
 Fixpoint Inb `{H : EqClass ID_Type} (a:ASP_ID) (l:list ASP_ID) : bool :=
   match l with
-    | [] => false
-    | b :: m => orb (eqb b a) (Inb a m)
+  | [] => false
+  | b :: m => orb (eqb b a) (Inb a m)
   end.
-
+  
+(** Within the manifest [m], does the AMß have ASP [a]? *)
 Definition hasASPm (m:Manifest) (a:ASP_ID) : bool :=
   Inb a m.(asps).  
 
+(* same consideration but with the environment *)
 Definition hasASPe(k:Plc)(e:Environment)(a:ASP_ID) : bool :=
 match (e k) with
 | None => false
 | Some m => Inb a m.(asps)
 end.      
 
-(** Determine if manifest [k] from [e] knows how to 
-   communicate from [k] to [p]
-*)
-
+(** Determine if manifest [m] knows how to communicate with [k] *)
 Definition knowsOfm (m:Manifest) (k:Plc) : bool :=
   Inb k m.(knowsOf).
-
+  
+(** Determine if manifest [k] from [e] knows how to communicate from [k] to [p] *)
 Definition knowsOfe `{H: EqClass ID_Type} (k:Plc)(e:Environment)(p:Plc): bool :=
 match (e k) with
 | None => false
@@ -122,7 +114,8 @@ end.
   place's manifest. Without the enviornment, we have no way 
   of knowing what place belongs to what Manifest. We could
   make manifests place dependent but I'm not sure we want to
-  do that...  *)
+  do that...  
+  Will says forgo this for now.... *)
 Fixpoint executable (t:Term) (m:Manifest): bool :=
 match t with
 | asp a  => match a with 
@@ -145,6 +138,7 @@ end.
 *        POLICY
 *******************************)
 
+(** Check manifest [m] and see if place [p] can run a. *)
 Definition checkMPolicy (p:Plc) (m:Manifest) (a:ASP_ID) : bool := 
   policy m a p.  
 
@@ -160,19 +154,17 @@ end.
 Fixpoint checkTermPolicy(t:Term)(k:Plc)(m:Manifest): bool :=
   match t with
   | asp a  => match a with 
-              | ASPC _ _ p => match p with 
-                              | asp_paramsC aspid _ _ _ => hasASPe k e aspid
-                              end
+              | ASPC _ _ (asp_paramsC aspid _ _ _ )=> checkMPolicy k m aspid
               | NULL => true
               | CPY => true
               | SIG => true
               | HSH => true
               | ENC p => true
               end
-  | att r t0 => checkTermPolicy t0 k e
-  | lseq t1 t2 => andb (checkTermPolicy t1 k e) (checkTermPolicy t2 k e)
-  | bseq _ t1 t2 => andb (checkTermPolicy t1 k e) (checkTermPolicy t2 k e)
-  | bpar _ t1 t2 => andb (checkTermPolicy t1 k e) (checkTermPolicy t2 k e)
+  | att r t0 => checkTermPolicy t0 k m
+  | lseq t1 t2 => andb (checkTermPolicy t1 k m) (checkTermPolicy t2 k m)
+  | bseq _ t1 t2 => andb (checkTermPolicy t1 k m) (checkTermPolicy t2 k m)
+  | bpar _ t1 t2 => andb (checkTermPolicy t1 k m) (checkTermPolicy t2 k m)
   end.
 
 (*****************************
@@ -182,64 +174,50 @@ Fixpoint checkTermPolicy(t:Term)(k:Plc)(m:Manifest): bool :=
 (** Soundness is executability and policy adherence *)
 
 Definition sound (t:Term)(m:Manifest) (k:Plc) :=
-  andb (executable t m) (checkTermPolicy t k e).
+  andb (executable t m) (checkTermPolicy t k m).
+
+(*****************************
+ * NEGOTIATION
+ *****************************)
+
+(* Negotiate' 
+   * input : t is list of requested terms 
+             r is list of proposed terms 
+   * output : list of proposed terms 
+   * reasoning: check if requested term satisfies soundness
+                the soundness check is done  *)
+
+Fixpoint negotiate' (t: list Term ) (r: list Term) (m: Manifest) (tp : Plc): list Term := 
+  match t with 
+  | [] => r
+  | h :: tl => if sound h m tp then negotiate' tl ([h] ++ r) m tp else negotiate' tl r m tp
+  end.
 
 (** ***************************
  * DEMO SYSTEM 
  *****************************)
 
-(* the target should be able to share: 
-   1. kim_meas_aspid wiht kim_meas_targid
-   2. the cal_ak_aspid with cal_ak_targid 
-   3. the public key to bc (?)
-   4. data 
-   5. tpm signature
-   6. ssl encryption *)
+ Definition server_plc := dest_plc.
+ Definition client_plc := source_plc.
 
-   (* might want to care who it discloses evidence to *)
-Inductive server_Policy : ASP_ID -> Plc -> Prop := 
-| p_kim : server_Policy kim_meas_aspid kim_meas_targid 
-| p_cal_ak : server_Policy cal_ak_aspid cal_ak_targid
-| p_pub_bc : server_Policy pub_bc_aspid pub_bc_targid
-| p_data : server_Policy get_data_aspid get_data_targid
-| p_tpm_sig : server_Policy tpm_sig_aspid tpm_sig_targid 
-| p_ssl_enc : server_Policy ssl_enc_aspid ssl_enc_targid. 
-
-(* Definition server_Policy_bool : forall a p, reflect (server_Policy a p). *)
+(* the server should be able to share: 
+   1. kim_meas_aspid with client  *)
 
 Notation "x && y" := (andb x y).
 Notation "x || y" := (orb x y).
 
 (* server can share data with source_plc (client) *)
 Definition server_Policy_bool  `{H : EqClass ID_Type} (a: ASP_ID) (p:Plc) : bool := 
-    (eqb a kim_meas_aspid && eqb p source_plc) || 
-    (eqb a cal_ak_aspid && eqb p source_plc) || 
-    (eqb a pub_bc_aspid && eqb p source_plc) || 
-    (eqb a get_data_aspid && eqb p source_plc) ||
-    (eqb a tpm_sig_aspid && eqb p source_plc) || 
-    (eqb a ssl_enc_aspid && eqb p source_plc) .
+    (eqb a kim_meas_aspid && eqb p client_plc).
 
     (* client can share data with dest_plc (server) *)
 Definition client_Policy_bool `{H : EqClass ID_Type} (a: ASP_ID) (p:Plc) : bool := 
- (eqb a store_clientData_aspid && eqb p dest_plc).
+ (eqb a store_clientData_aspid && eqb p server_plc).
 
-(** Definition of environments for use in examples and proofs.  
- * Note there are 2 communicating peer's present... server and client
- * About the demo:  
- ** client is source_plc 
- ** server is dest_plc
- ** client is appraising the server 
- *)
+(** Definition of manifest for use in examples and proofs. *)
 
-Definition e0 := e_empty.
-Definition e_client :=
-    e_update e0 source_plc (Some {| asps := [store_clientData_aspid]; knowsOf:= [dest_plc] ; context := [] ; policy := client_Policy_bool |}).
-Definition e_server :=
-    e_update e0 dest_plc (Some {| asps := [kim_meas_aspid;  cal_ak_aspid; pub_bc_aspid; get_data_aspid; tpm_sig_aspid; ssl_enc_aspid]; knowsOf:= [] ; context := [] ; policy := server_Policy_bool|}).
-
-(** In our example, the system includes client and server *)
-
-Definition example_sys_1 := [ e_client; e_server]. 
+Definition m_client := ({| asps := [store_clientData_aspid]; knowsOf:= [dest_plc] ; context := [] ; policy := client_Policy_bool |}).
+Definition m_server := ({| asps := [kim_meas_aspid;  cal_ak_aspid; pub_bc_aspid; get_data_aspid; tpm_sig_aspid; ssl_enc_aspid]; knowsOf:= [] ; context := [] ; policy := server_Policy_bool|}).
 
 (** ***************************
   * EXAMPLE SYSTEM PROPERTIES
@@ -264,20 +242,21 @@ Ltac eqbr var :=
   assert (H : (let (eqb, _) := Eq_Class_ID_Type in eqb) var
   var = true); [eapply eqb_refl |]; rewrite H.
   
-(** Prove the P0 knows of P1 in P0's enviornment *)
-
-Example ex1 : knowsOfe source_plc e_client dest_plc = true.
-Proof.
+(** Prove client knows of server *)
+Example ex1 : knowsOfm m_client server_plc = true.
+Proof. 
   cbv.
-  eqbr source_plc.
   eqbr dest_plc.
   eauto.
 Qed.
 
+(* demo phrase currently is a kim measurement *)
+Definition demo_phrase := kim_meas.
+Print kim_meas. (* <{ << kim_meas_aspid dest_plc kim_meas_targid >> }> *)
+
 (** Prove server can share kim_meas (the demo phrase) with the client. 
     AKA that it satisfies policy *)
-
-Theorem kim_meas_policy : server_Policy_bool kim_meas_aspid source_plc = true.
+Theorem kim_meas_policy : server_Policy_bool kim_meas_aspid client_plc = true.
 Proof.
   cbv. 
   eqbr kim_meas_aspid.
@@ -285,51 +264,9 @@ Proof.
   auto. 
 Qed.
 
-
-(* Remove all other theorems for now.... *)
-
-(* Steps for negotiation 
-   1. pass in protocol 
-   2. check executability and soundness
-   3. return protocol if passes check *)
-
-Print sound. 
-
-(* Negotiate' 
-   * input : t is list of requested terms 
-             r is list of proposed terms 
-   * output : list of proposed terms 
-   * reasoning: check if requested term satisfies soundness
-                the soundness check is done  *)
-
-Fixpoint negotiate' (t: list Term ) (r: list Term): list Term := 
-  match t with 
-  | [] => r
-  | h :: tl => if sound h dest_plc e_server then negotiate' tl ([h] ++ r) else negotiate' tl r 
-  end.
-
-
-(* Negotiate. 
-   * input: list of terms. This is the request. 
-   * output : list of terms. This is the proposal. 
-   * reasoning: pass input to helper function negotiate 
-       to call soundness check with empty list as proposal *)  
-Definition negotiate (t:list Term) : list Term := 
-  negotiate' t []. 
-
-(* demo phrase currently is a kim measurement *)
-Definition demo_phrase := kim_meas.
-
-Theorem negotiate_demo : negotiate [demo_phrase] = [kim_meas].
+Theorem demo_phrase_checkMPolicy : checkMPolicy server_plc m_server kim_meas_aspid = true.
 Proof.
-  cbv. 
-  eqbr dest_plc.
+  cbv.
   eqbr kim_meas_aspid.
-  auto.
-Qed. 
 
-Definition selection (t : list Term) : option Term := 
-match t with 
-| [] => None 
-| h :: tl => Some h 
-end. 
+
